coeToUniv_mem_iff' ...이게 문제였구나

Nemonuri/FinsetLike.lean
@@ -5,7 +5,18 @@ public import Mathlib.Data.Fintype.Basic
 
 @[expose] public section
 
+--def Equiv.Finset.univ {α: Type _} [Fintype α] : α ≃ (.univ: Finset α) where
+--  toFun
+
+
 namespace Nemonuri
+
+@[simps]
+def finsetUnivEquiv {α: Type _} [Fintype α] : α ≃ (.univ: Finset α) where
+  toFun x := ⟨x, Finset.mem_univ x⟩
+  invFun x := x.val
+
+--#print Nemonuri.finsetUnivEquiv_apply_coe
 
 class FinsetLike (A: Type _) (B: outParam <| Type _) where
   protected coe : A → Finset B
@@ -17,11 +28,18 @@ namespace FinsetLike
 
 variable {A: Type _} {B: Type _} [FinsetLike A B]
 
-instance : CoeOut A (Finset B) where coe := FinsetLike.coe
+instance : CoeHead A (Finset B) where coe := FinsetLike.coe
 
+/-
 instance : SetLike A B where
   coe a := FinsetLike.coe a
   coe_injective a1 a2 := by simp [FinsetLike.coe_injective.eq_iff]
+-/
+
+theorem finset_mem_iff_set_mem (A B: Type _) [FinsetLike A B] (a: A) (b: B)
+  : b ∈ (a: Finset B) ↔ b ∈ (a: Set B) := by
+  rfl
+  --rfl
 
 
 instance {α: Type _} : FinsetLike (Finset α) α where
@@ -46,12 +64,38 @@ instance {α: Type _} (fs: Finset α) : FinsetLike (fs → Bool) fs where
   coe := coeBoolPredFor fs
   coe_injective := coeBoolPredFor_injective fs
 
+/-
 instance {α: Type _} [Fintype α] : FinsetLike (Fintype α) α where
   coe _ := Finset.univ
   coe_injective ft1 ft2 _ := Fintype.subsingleton α |>.allEq ft1 ft2
+-/
+
+instance {α: Type _} [Fintype α] : FinsetLike (α → Bool) α where
+  coe f := (.univ: Finset α).filter (f · = .true)
+  coe_injective f1 f2 := by
+    simp only
+    intro lm1
+    simp [SetLike.ext_iff] at lm1
+    ext x
+    exact lm1 x
 
 
-theorem fintype_coe_eq_univ {α: Type _} [ft: Fintype α] : (ft: Finset α) = Finset.univ := rfl
+instance coeToUniv {α: Type _} [Fintype α] : FinsetLike (Finset α) (.univ: Finset α) where
+  coe fs := fs.map finsetUnivEquiv.toEmbedding
+  coe_injective fs1 fs2 := by
+    simp only [Finset.map_inj]
+    exact id
+
+theorem coeToUniv_mem_iff {α: Type _} [Fintype α] (fs: Finset α) (a: α)
+  : (finsetUnivEquiv a) ∈ ((@coeToUniv α _).coe fs) ↔ a ∈ fs := by
+  unfold coeToUniv
+  simp only [Finset.mem_map_mk]
+
+@[simp]
+theorem coeToUniv_mem_iff' {α: Type _} [Fintype α] (fs: Finset α) (a: (.univ: Finset α))
+  : a ∈ ((@coeToUniv α _).coe fs) ↔ (a.val) ∈ fs := by
+  unfold coeToUniv
+  simp only [Finset.mem_map_equiv, finsetUnivEquiv_symm_apply]
 
 
 end FinsetLike
